#### Assembly
```
cpy a d
cpy 4 c
cpy 633 b
inc d
dec b
jnz b -2
dec c
jnz c -5
cpy d a
jnz 0 0
cpy a b
cpy 0 a
cpy 2 c
jnz b 2
jnz 1 6
dec b
dec c
jnz c -4
inc a
jnz 1 -7
cpy 2 b
jnz c 2
jnz 1 4
dec b
dec c
jnz 1 -4
jnz 0 0
out b
jnz a -19
jnz 1 -21
```

#### Disassembled
```
    D = A
    C = 4
L2:
    B = 633 <-----------------+   D += 633 * C
L1:                           |
    D += 1  <---------------+ |
    B -= 1                  | |
    if (B != 0) goto L1 ----+ |
    C -= 1                    |
    if (C != 0) goto L2 ------+
L11:
    A = D    <-----------------------------+
L10:                                       |
    B = A    <---------------------------+ |
    A = 0                                | |
L6:                                      | |
    C = 2  <------------------------+    | |
L5:                                 |    | |
    if (B != 0) goto L3 ----+  <--+ |    | |
    goto L4 --------------+ |     | |    | |
L3:                       | |     | |    | |
    B -= 1  <---------------+     | |    | |
    C -= 1                |       | |    | |
    if (C != 0) goto L5 --|-------+ |    | |
    A += 1                |         |    | |
    goto L6 --------------|---------+    | |
L4:                       |              | |
    B = 2  <--------------+              | |
L9:                                      | |
    if (C != 0) goto L7 --+ <--+         | |
    goto L8 -----+        |    |         | |
L7:              |        |    |         | |
    B -= 1 <--------------+    |         | |
    C -= 1       |             |         | |
    goto L9 -----|-------------+         | |
L8:              |                       | |
    out B <------+                       | |
    if (A != 0) goto L10: ---------------+ |
    goto L11 ------------------------------+
```


#### Decompilation

```C
D = A + 633 * 4;
A = D;

while (true) {

    B = A;
    A = 0;

    C = 2;
    while (B) {
        B--;
        C--;
        if (!C) {
            A++;
            C = 2;
        }
    }

    B = 2;
    while (C) {
        B--;
        C--;
    }

    output(B)

    if (!A) A = D;

}
```

#### Simplified Decompilation
```C
A += 633 * 4
D = A

while (true) {

    // 1

    B = A % 2;
    A /= 2;

    // 2

    output(B);

    if (!A) A = D;

}
```

#### Solution

```C
A2 = 0  -->  A1 = 1  -->  B = 1  // n = 1
A2 = 1 && B = 0  -->  A1 = 2     // n = 2
A2 = 2 && B = 1  -->  A1 = 5     // n = 3
A2 = 5 && B = 0  -->  A1 = 10    // n = 4
A2 = 10 && B = 1  --> A1 = 21    // n = 5
...
A1 = (- 3 + 2^(n + 2) - (-1)^n) / 6
...
A1 = A + 2532 && A1 % 2 = 0 // A is even, n must be even
```

$$
A = \frac{1}{6}(- 3 + 2^{(n + 2)} - (-1)^n) - 2532 \\
\frac{1}{6}(2^{(n + 2)} - 4) \ge 2532 \\
2^{(n + 2)} - 4 \ge 15192 \\
n + 2 \ge \log_2(15196) \\
n \ge \log_2(15196) - 2 \\
n \ge 11.8914039967... \\
n = 12 \\
A = \frac{1}{6}(2^{(12 + 2)} - 4) - 2532 \\
A = 198
$$